\include{header}
\newcommand{\Mac}{\mathfrak{M}}
\DeclareMathOperator{\type}{type}
\begin{document}
%\section{Expanding a power-sum MacMahon symmetric function in the monomial basis}
%\bigskip
%
%Fix a positive integer $r$.  Throughout, we will work with MacMahon symmetric functions in $r$ alphabets.  The complete set of variables is
%\[\{x_{i,j}\mid i\in\Pp,\ j\in[r]\}.\]
%
%Fix vector partitions $\lambda=(\lambda_1,\dots,\lambda_\ell)$ and $\mu=(\mu_1,\dots,\mu_m)$ of the same vector, where
%\begin{align*}
%\lambda_i&=(\lambda_{i,1},\dots,\lambda_{i,r})\in\Pp^r\setminus\{\vec0\},\\
%\mu_i&=(\mu_{i,1},\dots,\mu_{i,r})\in\Pp^r\setminus\{\vec0\}.
%\end{align*}
%
%The monomial MacMahon symmetric function indexed by $\mu$ is the sum of all monomials in the diagonal $\mathfrak{S}_n$-orbit of the monomial
%\[x_\mu = \prod_{i=1}^m \prod_{j=1}^r x_{i,j}^{\mu_{i,j}}.\]
%
%The power-sum MacMahon symmetric function indexed by $\lambda$ is
%\begin{align*}
%P_\lambda
%&= \prod_{i=1}^\ell P_{\lambda_i}\\
%&= \prod_{i=1}^\ell \sum_{k\in\Pp} x_{k,1}^{\lambda_{i,1}}\cdots x_{k,r}^{\lambda_{i,r}}\\
%&= \sum_{(k_1,\dots,k_\ell)\in\Pp^\ell} \prod_{i=1}^\ell x_{k_i,1}^{\lambda_{i,1}}\cdots x_{k_i,r}^{\lambda_{i,r}}.
%\end{align*}
%
%Thus the coefficient of $x_\mu$ in $P_\lambda$ is
%\[\#\left\{(k_1,\dots,k_\ell)\in\Pp^\ell \mid \sum_{i\colon\,k_i=h}\lambda_i=\mu_h\ \ \forall h\in[m]\right\}.\]
%Note that we can replace $\Pp^\ell$ by $m^\ell$.
%
%For example, fix $r=2$.  Let $\mu=(1,1)(1,2)$, so that
%\[x_\mu = x_{1,1}^1 x_{1,2}^1 x_{2,1}^1 x_{2,2}^2\]
%and let $\lambda=(1,1)(1,0)(0,1)(0,1)$ so that $\ell=4$ and
%\begin{align*}
%P_\lambda
%&= \sum_{(k_1,\dots,k_4)} \prod_{i=1}^4 x_{k_i,1}^{\lambda_{i,1}} x_{k_i,2}^{\lambda_{i,2}}\\
%&= \sum_{(k_1,\dots,k_4)} 
%x_{k_1,1}^{\lambda_{1,1}} x_{k_1,2}^{\lambda_{1,2}}
%x_{k_2,2}^{\lambda_{2,1}} x_{k_2,2}^{\lambda_{2,2}}
%x_{k_3,1}^{\lambda_{3,1}} x_{k_3,2}^{\lambda_{3,2}}
%x_{k_4,1}^{\lambda_{4,1}} x_{k_4,2}^{\lambda_{4,2}}\\
%&= \sum_{(k_1,\dots,k_4)} 
%x_{k_1,1}^1 x_{k_1,2}^1
%x_{k_2,2}^1 x_{k_2,2}^0
%x_{k_3,1}^0 x_{k_3,2}^1
%x_{k_4,1}^0 x_{k_4,2}^1
%\end{align*}
%so in order to make this monomial equal to $x_\mu$, we need
%\[\sum_{i:\ k_i=1} \lambda_i = \mu_1 = (1,1),
%\qquad\sum_{i:\ k_i=2} \lambda_i = \mu_2 = (1,2).\]
%The solutions for $(k_1,k_2,k_3,k_4)$ and the corresponding expressions for $x_\mu$ are
%\begin{align*}
%(1,2,2,2) & & x_{1,1}^1 x_{1,2}^1 x_{2,1}^1 x_{2,2}^2 &= (x_{1,1}^1 x_{1,2}^1)(x_{2,2}^1 x_{2,2}^0)(x_{2,1}^0 x_{2,2}^1)(x_{2,1}^0 x_{2,2}^1)\\
%(2,1,1,2) & & x_{1,1}^1 x_{1,2}^1 x_{2,1}^1 x_{2,2}^2 &= (x_{2,1}^1 x_{2,2}^1)(x_{1,2}^1 x_{1,2}^0)(x_{1,1}^0 x_{1,2}^1)(x_{2,1}^0 x_{2,2}^1)\\
%(2,1,2,1) & & x_{1,1}^1 x_{1,2}^1 x_{2,1}^1 x_{2,2}^2 &= (x_{2,1}^1 x_{2,2}^1)(x_{1,2}^1 x_{1,2}^0)(x_{2,1}^0 x_{2,2}^1)(x_{1,1}^0 x_{1,2}^1)\\
%\end{align*}
%So the coefficient is 3.  This could certainly be calculated algorithmically.
%

\section{Transitions between bases [Rosas 2001]}

First, a standard linear algebra fact.
Let $V$ be a vector space of finite dimension~$n$ over ground field $\Bbbk$ (it doesn't matter what it is).

\begin{proposition} \label{expansion}
Suppose that $B=\{v_1,\dots,v_n\}$ and $B^*=\{v_1^*,\dots,v_n^*\}$ are bases for $V$ that are orthogonal, i.e.,
\[\langle v_i,v^*_j\rangle=\delta_{ij} k_i\]
for some nonzero constants $k_1,\dots,k_n$.  Then the unique expansion of $u$ with respect to $B$ is
\begin{equation} \label{expand-in-basis}
u = \sum_{i=1}^n \frac{\langle v_i^*,\,u\rangle}{k_i} v_i.
\end{equation}
\end{proposition}

\begin{proof}
For every $j\in[n]$ we have
\[
\left\langle v_j^*,\ \sum_{i=1}^n \frac{\langle v_i^*,\,u\rangle}{k_i} v_i\right\rangle
= \sum_{i=1}^n \frac{\langle v_i^*,\,u\rangle}{k_i} \langle v_j^*,\,v_i\rangle
= \sum_{i=1}^n \langle v_i^*,\,u\rangle \delta_{ij}
= \langle v_j^*,\,u\rangle.\]
That is, every element of $B^*$ has the same inner product with the left and right-hand sides of~\eqref{expand-in-basis}.
This is necessary and sufficient for equality.
\end{proof}

This proposition reduces the problem of expanding a vector in a particular basis $B$ to computing inner products with an orthogonal basis $B^*$.
(The best possible case is that $k_i=1$ for all $i$, i.e., $B^*$ is the dual basis to $B$.  However, we're not always that lucky.)


Notation:
\begin{itemize}
\item $\Nn$ = nonnegative integers;
\item For $u\in\Nn^k$, a \textbf{vector partition} $\lambda\partn u$ is an unordered sequence of vectors (\textbf{parts}) summing to $u$; zero vectors can be ignored.
\item Weight of a vector partition = sum of all entries in all vectors in it (ex.: $\wt(\{120,100,100,013\})=9$)
\item $\Mac_\uu$ = MacMahon symmetric functions of homogeneous multidegree $u$
\item $\sign(\lambda)=(-1)^{\text{number of parts with even sum}}$
\item $m_\lambda,e_\lambda,h_\lambda,p_\lambda,f_\lambda$: monomial, elementary, homogeneous, power-sum, and forgotten MacMahon symmetric functions (Rosas 327--328)
\item For a vector partition $\lambda$ in which each part $v_i$ occurs with multiplicity $m_i$, define
\[|\lambda|=\prod_im_i! \qqandqq \lambda!=\prod_i\prod_{x\in v_i}(x!)^{m_i}.\]
\end{itemize}

A vector partition is \textbf{unitary} if it is a partition of the all-ones vector $\mathbf{1}\in\Nn^k$.  There is an obvious bijection between unitary vector partitions and set partitions of $[k]$.  There is a whole theory of MacMahon symmetric functions of unitary partitions, due to Doubilet.  These are the graded pieces $\Mac_{(1)^k}$.

The \textbf{type} of a set partition $\pi=B_1|\cdots|B_\ell$, with respect to a vector $u=(u_1,\dots,u_r)$ of weight $n$, is the vector partition $\type_\uu(\pi)=\lambda=\lambda_1\cdots\lambda_\ell$ where $\lambda_k$ is the vector in $\Nn^r$ whose $i$th coordinate is
\[\#\{j\in B_k \mid u_1+\cdots+u_{i-1} < j \leq i_1+\cdots+u_i\}.\]
 the number of elements of $B_k$ such that
in the $i$th equivalence class.

For a vector $u$ of weight $n$ and a vector partition $\lambda$ of weight $n$, the number of set partitions $\pi$ of type $\type_\uu(\pi)$ is
\[\binom{u}{\lambda} := \frac{u!}{\lambda!\,|\lambda|}.\]

Define a scalar product on $\Mac$:
\begin{equation}\label{scalar-product}
\boxed{\scp{h_\lambda}{m_\mu}=\delta_{\lambda\mu}.}
\end{equation}
The idea is to use this for basis transitions, along the lines discussed earlier.  Specifically, formula~\eqref{expand-in-basis} says that for any $F\in\Mac_\uu$, we have
\begin{equation} \label{expand-Mac}
F=\sum_{\lambda\partn u} \langle h_\lambda,\,F\rangle m_\lambda \qqandqq
F=\sum_{\lambda\partn u} \langle m_\lambda,\,F\rangle h_\lambda.
\end{equation}

Thus we have to know how to compute inner products.

There is a ``lifting map'' $\hat\rho$ [Rosas 2001, Defn.~6] sending MacMahon functions to unitary (Doubilet) symmetric functions.  Specifically:
\begin{subequations}
\begin{align}
\binom{\uu}{\lambda}|\lambda|\,m_\lambda &\overset{\hat\rho}{\longmapsto} \sum_{\pi\colon \type_\uu(\pi)=\lambda} m_\pi \label{liftM}\\
\binom{\uu}{\lambda}\lambda!\,h_\lambda &\overset{\hat\rho}{\longmapsto} \sum_{\pi\colon \type_\uu(\pi)=\lambda} h_\pi\label{liftH}\\
\binom{\uu}{\lambda}\lambda!\,e_\lambda &\overset{\hat\rho}{\longmapsto} \sum_{\pi\colon \type_\uu(\pi)=\lambda} e_\pi\label{liftE}\\
\binom{\uu}{\lambda}\,p_\lambda &\overset{\hat\rho}{\longmapsto} \sum_{\pi\colon \type_\uu(\pi)=\lambda} p_\pi\label{liftP}\\
\binom{\uu}{\lambda}|\lambda|\,f_\lambda &\overset{\hat\rho}{\longmapsto} \sum_{\pi\colon \type_\uu(\pi)=\lambda} f_\pi\label{liftF}
\end{align}
\end{subequations}

Moreover, for all $f,g\in\Mac_\uu$ we have
\begin{equation} \label{Rosas-scalar}
\scp{f}{g}=\uu!\scp{\hat\rho(f)}{\hat\rho(g)}
\end{equation}
[Rosas, Prop.~7].

Prop.~\ref{expansion} together with the scalar product~\eqref{scalar-product} says in particular that for $F\in\Mac_\uu$ we have
\begin{equation} \label{expand-HM}
F = \sum_{\lambda\partn\uu} \langle m_\lambda,\,F\rangle\, h_\lambda,
\qquad\qquad
F = \sum_{\lambda\partn\uu} \langle h_\lambda,\,F\rangle\, m_\lambda.
\end{equation}
Doubilet (Appendix 2) calculated the scalar products for all five families of unitary symmetric functions (which requires things like lattice operations and  M\"obius and zeta functions in the set partition lattice $\Pi_n$).  Therefore, we should be able to compute scalar products, and thus basis expansions, for all MacMahon functions.  Rosas reproduced Doubilet's calculations (in modern notation).

\section{Expansions in the $m$-basis}

\begin{align*}
p_\mu &=  \uu! \sum_{\lambda\partn\uu} \langle \hat\rho(h_\lambda),\,\hat\rho(p_\mu)\rangle\, m_\lambda
	&&\text{(by~\eqref{expand-Mac} and~\eqref{Rosas-scalar})}\\
&=  \uu! \sum_{\lambda\partn\uu} \left\langle \frac{1}{\binom{\uu}{\lambda}\lambda!} \sum_{\pi\colon \type_\uu(\pi)=\lambda} h_\pi, \ \ \frac{1}{\binom{\uu}{\mu}} \sum_{\sigma\colon \type_\uu(\sigma)=\mu} p_\sigma \right\rangle\, m_\lambda
	&&\text{(by~\eqref{liftH} and~\eqref{liftP})}\\
&=  \frac{\uu!}{\binom{\uu}{\mu}} \sum_{\lambda\partn\uu} \frac{1}{\binom{\uu}{\lambda}\lambda!}
    \sum_{\substack{\pi\colon \type_\uu(\pi)=\lambda\\ \sigma\colon \type_\uu(\sigma)=\mu}}
    \left\langle h_\pi,\,p_\sigma \right\rangle\, m_\lambda
	&&\text{(by bilinearity)}\\
&=  \frac{\uu!}{\binom{\uu}{\mu}} \sum_{\lambda\partn\uu} \frac{1}{\binom{\uu}{\lambda}\lambda!}
    \sum_{\substack{\pi\colon \type_\uu(\pi)=\lambda\\ \sigma\colon \type_\uu(\sigma)=\mu}}
    \zeta(\sigma,\pi) m_\lambda
	&&\text{(by~Doubilet formula \#3)}\\
p_\mu &= \boxed{ \frac{\uu!}{\binom{\uu}{\mu}} \sum_{\lambda\partn\uu} \frac{\#\{(\pi,\sigma)\mid \type_\uu(\pi)=\lambda,\ \type_\uu(\sigma)=\mu,\ \sigma\leq\pi\}}{\binom{\uu}{\lambda}\lambda!}
    m_\lambda}
\end{align*}

\begin{align*}
h_\mu &=  \uu! \sum_{\lambda\partn\uu} \langle \hat\rho(h_\lambda),\,\hat\rho(h_\mu)\rangle\, m_\lambda
	&&\text{(by~\eqref{expand-Mac} and~\eqref{Rosas-scalar})}\\
&=  \uu! \sum_{\lambda\partn\uu} \left\langle \frac{1}{\binom{\uu}{\lambda}\lambda!} \sum_{\pi\colon \type_\uu(\pi)=\lambda} h_\pi, \ \ \frac{1}{\binom{\uu}{\mu}\mu!} \sum_{\sigma\colon \type_\uu(\sigma)=\mu} h_\sigma \right\rangle\, m_\lambda
	&&\text{(by~\eqref{liftH} twice)}\\
&=  \frac{\uu!}{\binom{\uu}{\mu}\mu!} \sum_{\lambda\partn\uu} \frac{1}{\binom{\uu}{\lambda}\lambda!}
    \sum_{\substack{\pi\colon \type_\uu(\pi)=\lambda\\ \sigma\colon \type_\uu(\sigma)=\mu}}
    \left\langle h_\pi,\,h_\sigma \right\rangle\, m_\lambda
	&&\text{(by bilinearity)}\\
&=  \frac{\uu!}{\binom{\uu}{\mu}\mu!} \sum_{\lambda\partn\uu} \frac{1}{\binom{\uu}{\lambda}\lambda!}
    \sum_{\substack{\pi\colon \type_\uu(\pi)=\lambda\\ \sigma\colon \type_\uu(\sigma)=\mu}}
    \lambda(\sigma\meet\pi)!\, m_\lambda
	&&\text{(by Doubilet formula \#9)}\\
\end{align*}

\begin{align*}
e_\mu &=  \uu! \sum_{\lambda\partn\uu} \langle \hat\rho(h_\lambda),\,\hat\rho(e_\mu)\rangle\, m_\lambda
	&&\text{(by~\eqref{expand-Mac} and~\eqref{Rosas-scalar})}\\
&=  \uu! \sum_{\lambda\partn\uu} \left\langle \frac{1}{\binom{\uu}{\lambda}\lambda!} \sum_{\pi\colon \type_\uu(\pi)=\lambda} h_\pi, \ \ \frac{1}{\binom{\uu}{\mu}\mu!} \sum_{\sigma\colon \type_\uu(\sigma)=\mu} e_\sigma \right\rangle\, m_\lambda
	&&\text{(by~\eqref{liftH} and~\eqref{liftE})}\\
&=  \frac{\uu!}{\binom{\uu}{\mu}\mu!} \sum_{\lambda\partn\uu} \frac{1}{\binom{\uu}{\lambda}\lambda!}
    \sum_{\substack{\pi\colon \type_\uu(\pi)=\lambda\\ \sigma\colon \type_\uu(\sigma)=\mu}}
    \left\langle h_\pi,\,e_\sigma \right\rangle\, m_\lambda
	&&\text{(by bilinearity)}\\
&=  \frac{\uu!}{\binom{\uu}{\mu}\mu!} \sum_{\lambda\partn\uu} \frac{\#\{(\pi,\sigma)\mid \type_\uu(\pi)=\lambda,\ \type_\uu(\sigma)=\mu,\ \pi\meet\sigma=\hatzero\}}{\binom{\uu}{\lambda}\lambda!} m_\lambda
	&&\text{(by Doubilet formula \#6)}\\
\end{align*}

\begin{align*}
f_\mu &=  \uu! \sum_{\lambda\partn\uu} \langle \hat\rho(h_\lambda),\,\hat\rho(f_\mu)\rangle\, m_\lambda
	&&\text{(by~\eqref{expand-Mac} and~\eqref{Rosas-scalar})}\\
&=  \uu! \sum_{\lambda\partn\uu} \left\langle \frac{1}{\binom{\uu}{\lambda}\lambda!} \sum_{\pi\colon \type_\uu(\pi)=\lambda} h_\pi, \ \ \frac{1}{\binom{\uu}{\mu}|\mu|} \sum_{\sigma\colon \type_\uu(\sigma)=\mu} f_\sigma \right\rangle\, m_\lambda
	&&\text{(by~\eqref{liftH} and~\eqref{liftP})}\\
&=  \frac{\uu!}{\binom{\uu}{\mu}|\mu|} \sum_{\lambda\partn\uu} \frac{1}{\binom{\uu}{\lambda}\lambda!}
    \sum_{\substack{\pi\colon \type_\uu(\pi)=\lambda\\ \sigma\colon \type_\uu(\sigma)=\mu}}
    \left\langle h_\pi,\,f_\sigma \right\rangle\, m_\lambda
	&&\text{(by bilinearity)}\\
&=  \frac{\uu!}{\binom{\uu}{\mu}|\mu|} \sum_{\lambda\partn\uu} \frac{1}{\binom{\uu}{\lambda}\lambda!}
    \sum_{\substack{\pi\colon \type_\uu(\pi)=\lambda\\ \sigma\colon \type_\uu(\sigma)=\mu\\ \sigma\leq\pi}}
    \lambda(\sigma,\pi)!  m_\lambda
	&&\text{(by Doubilet formula \#13)}\\
\end{align*}

\section{Expansions in the $h$-basis}

\begin{align*}
m_\mu &=  \uu! \sum_{\lambda\partn\uu} \langle \hat\rho(m_\lambda),\,\hat\rho(m_\mu)\rangle\, h_\lambda
	&&\text{(by~\eqref{expand-Mac} and~\eqref{Rosas-scalar})}\\
&= \uu! \sum_{\lambda\partn\uu} \left\langle \frac{1}{\binom{\uu}{\lambda}|\lambda|} \sum_{\pi\colon \type_\uu(\pi)=\lambda} m_\pi, \ \ \frac{1}{\binom{\uu}{\mu}|\mu|} \sum_{\sigma\colon \type_\uu(\sigma)=\mu} m_\sigma \right\rangle\, h_\lambda
	&&\text{(by~\eqref{liftM} twice)}\\
&= \frac{\uu!}{\binom{\uu}{\mu}|\mu|} \sum_{\lambda\partn\uu} \frac{1}{\binom{\uu}{\lambda}|\lambda|}
    \sum_{\substack{\pi\colon \type_\uu(\pi)=\lambda\\ \sigma\colon \type_\uu(\sigma)=\mu}}
    \left\langle m_\pi,\ m_\sigma \right\rangle\, h_\lambda
	&&\text{(by bilinearity)}\\
&= \frac{\uu!}{\binom{\uu}{\mu}|\mu|} \sum_{\lambda\partn\uu} \frac{1}{\binom{\uu}{\lambda}|\lambda|}
    \sum_{\substack{\pi\colon \type_\uu(\pi)=\lambda\\ \sigma\colon \type_\uu(\sigma)=\mu}}
    \sum_{\tau\geq\pi\join\sigma} \frac{\mu(\pi,\tau)\mu(\sigma,\tau)}{\mu(\hatzero,\tau)}\, h_\lambda
	&&\text{(by Doubilet formula \#7)}\\
\end{align*}

\begin{align*}
p_\mu &=  \uu! \sum_{\lambda\partn\uu} \langle \hat\rho(m_\lambda),\,\hat\rho(p_\mu)\rangle\, h_\lambda
	&&\text{(by~\eqref{expand-Mac} and~\eqref{Rosas-scalar})}\\
&=  \uu! \sum_{\lambda\partn\uu} \left\langle \frac{1}{\binom{\uu}{\lambda}|\lambda|} \sum_{\pi\colon \type_\uu(\pi)=\lambda} m_\pi, \ \ \frac{1}{\binom{\uu}{\mu}} \sum_{\sigma\colon \type_\uu(\sigma)=\mu} p_\sigma \right\rangle\, h_\lambda
	&&\text{(by~\eqref{liftM} and~\eqref{liftP})}\\
&= \frac{\uu!}{\binom{\uu}{\mu}} \sum_{\lambda\partn\uu} \frac{1}{\binom{\uu}{\lambda}|\lambda|}
    \sum_{\substack{\pi\colon \type_\uu(\pi)=\lambda\\ \sigma\colon \type_\uu(\sigma)=\mu}}
    \left\langle m_\pi,\ p_\sigma \right\rangle\, h_\lambda
	&&\text{(by bilinearity)}\\
&= \frac{\uu!}{\binom{\uu}{\mu}} \sum_{\lambda\partn\uu} \frac{1}{\binom{\uu}{\lambda}|\lambda|}
    \sum_{\substack{\pi\colon \type_\uu(\pi)=\lambda\\ \sigma\colon \type_\uu(\sigma)=\mu\\ \pi\leq\sigma}}
    \frac{\mu(\pi,\sigma)}{|\mu(\hatzero,\sigma)|}\, h_\lambda
	&&\text{(by Doubilet formula \#10)}\\
\end{align*}

\begin{align*}
e_\mu &=  \uu! \sum_{\lambda\partn\uu} \langle \hat\rho(m_\lambda),\,\hat\rho(e_\mu)\rangle\, h_\lambda
	&&\text{(by~\eqref{expand-Mac} and~\eqref{Rosas-scalar})}\\
&=  \uu! \sum_{\lambda\partn\uu} \left\langle \frac{1}{\binom{\uu}{\lambda}|\lambda|} \sum_{\pi\colon \type_\uu(\pi)=\lambda} m_\pi, \ \ \frac{1}{\binom{\uu}{\mu}\mu!} \sum_{\sigma\colon \type_\uu(\sigma)=\mu} e_\sigma \right\rangle\, h_\lambda
	&&\text{(by~\eqref{liftM} and~\eqref{liftE})}\\
&= \frac{\uu!}{\binom{\uu}{\mu}\mu!} \sum_{\lambda\partn\uu} \frac{1}{\binom{\uu}{\lambda}|\lambda|}
    \sum_{\substack{\pi\colon \type_\uu(\pi)=\lambda\\ \sigma\colon \type_\uu(\sigma)=\mu}}
    \left\langle m_\pi,\ e_\sigma \right\rangle\, h_\lambda
	&&\text{(by bilinearity)}\\
&= \frac{\uu!}{\binom{\uu}{\mu}\mu!} \sum_{\lambda\partn\uu} \frac{1}{\binom{\uu}{\lambda}|\lambda|}
    \sum_{\substack{\pi\colon \type_\uu(\pi)=\lambda\\ \sigma\colon \type_\uu(\sigma)=\mu\\ \pi\leq\sigma}}
    \sign(\pi) \lambda(\pi,\sigma)!\, h_\lambda
	&&\text{(by Doubilet formula \#8)}\\
\end{align*}

\begin{align*}
f_\mu &=  \uu! \sum_{\lambda\partn\uu} \langle \hat\rho(m_\lambda),\,\hat\rho(f_\mu)\rangle\, h_\lambda
	&&\text{(by~\eqref{expand-Mac} and~\eqref{Rosas-scalar})}\\
&=  \uu! \sum_{\lambda\partn\uu} \left\langle \frac{1}{\binom{\uu}{\lambda}|\lambda|} \sum_{\pi\colon \type_\uu(\pi)=\lambda} m_\pi, \ \ \frac{1}{\binom{\uu}{\mu}|\mu|} \sum_{\sigma\colon \type_\uu(\sigma)=\mu} f_\sigma \right\rangle\, h_\lambda
	&&\text{(by~\eqref{liftM} and~\eqref{liftF})}\\
&= \frac{\uu!}{\binom{\uu}{\mu}|\mu|} \sum_{\lambda\partn\uu} \frac{1}{\binom{\uu}{\lambda}|\lambda|}
    \sum_{\substack{\pi\colon \type_\uu(\pi)=\lambda\\ \sigma\colon \type_\uu(\sigma)=\mu}}
    \left\langle m_\pi,\ f_\sigma \right\rangle\, h_\lambda
	&&\text{(by bilinearity)}\\
&= \frac{\uu!}{\binom{\uu}{\mu}|\mu|} \sum_{\lambda\partn\uu} \frac{1}{\binom{\uu}{\lambda}|\lambda|}
    \sum_{\substack{\pi\colon \type_\uu(\pi)=\lambda\\ \sigma\colon \type_\uu(\sigma)=\mu}}
    \sum_{\tau\geq\sigma\join\pi} \frac{|\mu(\sigma,\tau)|\cdot\mu(\pi,\tau)}{\mu(\hatzero,\tau)}\, h_\lambda
	&&\text{(by Doubilet formula \#11)}\\
\end{align*}

\section{Expansions in the $p$-basis}

The power-sum basis is orthogonal (though not orthonormal).  A remark in Rosas (p.333) says that for $\lambda\partn\uu$,
\begin{equation}
\langle p_\lambda,\,p_\mu \rangle = \frac{\delta_{\lambda,\mu}|\lambda|\,\lambda!}{\mu(\hatzero,\lambda)}
\end{equation}
where $\mu(\hatzero,\lambda)$ means $\mu(\hatzero,\pi)$ for any set partition $\pi$ such that $\type_u(\pi)=\lambda$.

Therefore, Proposition~\ref{expansion} says that for every $F\in\Mac$,
\begin{equation} \label{expand-in-P-basis}
F = \sum_\lambda \frac{\langle p_\lambda,\,F\rangle \mu(\hatzero,\lambda)}{|\lambda|\,\lambda!} p_\lambda
= \sum_\lambda \frac{\langle p_\lambda,\,F\rangle \mu(\hatzero,\lambda) \binom{\uu}{\lambda}}{\uu!} p_\lambda
\end{equation}
So, as before:

\begin{align*}
m_\mu &= \sum_\lambda \left\langle \binom{\uu}{\lambda}\hat\rho(p_\lambda),\,\hat\rho(m_\mu)\right\rangle \mu(\hatzero,\lambda)  p_\lambda
	&&\text{(by~\eqref{expand-in-P-basis} and~\eqref{Rosas-scalar})}\\
&= \frac{1}{\binom{\uu}{\mu}|\mu|} \sum_\lambda \mu(\hatzero,\lambda) \sum_{\substack{\sigma\colon \type_\uu(\sigma)=\lambda\\ \pi\colon \type_\uu(\pi)=\mu}} \left\langle p_\sigma,\, m_\pi\right\rangle  p_\lambda
	&&\text{(by~\eqref{liftP} and~\eqref{liftM} and bilinearity)}\\
&= \frac{1}{\binom{\uu}{\mu}|\mu|} \sum_\lambda\left[ \mu(\hatzero,\lambda) \sum_{\substack{\sigma\colon \type_\uu(\sigma)=\lambda\\ \pi\colon \type_\uu(\pi)=\mu\\ \pi\leq\sigma}} \frac{\mu(\pi,\sigma)}{\mu(\hatzero,\sigma)} \right] p_\lambda
	&&\text{(by Doubilet formula \#10)}\\
\end{align*}

\begin{align*}
h_\mu &= \sum_\lambda \langle \hat\rho(p_\lambda),\,\hat\rho(h_\mu)\rangle \mu(\hatzero,\lambda) \binom{\uu}{\lambda} p_\lambda
	&&\text{(by~\eqref{expand-in-P-basis} and~\eqref{Rosas-scalar})}\\
&= \frac{1}{\binom{\uu}{\mu} \mu!} \sum_\lambda \mu(\hatzero,\lambda) \sum_{\substack{\sigma\colon \type_\uu(\sigma)=\lambda\\ \pi\colon \type_\uu(\pi)=\mu}} \left\langle p_\sigma,\, h_\pi\right\rangle  p_\lambda
	&&\text{(by~\eqref{liftP} and~\eqref{liftH} and bilinearity)}\\
&= \frac{1}{\binom{\uu}{\mu} \mu!} \sum_\lambda\left[ \mu(\hatzero,\lambda) \sum_{\substack{\sigma\colon \type_\uu(\sigma)=\lambda\\ \pi\colon \type_\uu(\pi)=\mu\\ \sigma\leq\pi}} \right] p_\lambda
	&&\text{(by Doubilet formula \#3)}\\
\end{align*}

\begin{align*}
e_\mu &= \sum_\lambda \langle \hat\rho(p_\lambda),\,\hat\rho(e_\mu)\rangle \mu(\hatzero,\lambda) \binom{\uu}{\lambda} p_\lambda
	&&\text{(by~\eqref{expand-in-P-basis} and~\eqref{Rosas-scalar})}\\
&= \frac{1}{\binom{\uu}{\mu} \mu!} \sum_\lambda \mu(\hatzero,\lambda) \sum_{\substack{\sigma\colon \type_\uu(\sigma)=\lambda\\ \pi\colon \type_\uu(\pi)=\mu}} \left\langle p_\sigma,\, e_\pi\right\rangle  p_\lambda
	&&\text{(by~\eqref{liftP} and~\eqref{liftE} and bilinearity)}\\
&= \frac{1}{\binom{\uu}{\mu} \mu!} \sum_\lambda\left[ \mu(\hatzero,\lambda) \sum_{\substack{\sigma\colon \type_\uu(\sigma)=\lambda\\ \pi\colon \type_\uu(\pi)=\mu\\ \sigma\leq\pi}} \sign(\sigma) \right] p_\lambda
	&&\text{(by Doubilet formula \#4)}\\
\end{align*}

\begin{align*}
f_\mu &= \sum_\lambda \langle \hat\rho(p_\lambda),\,\hat\rho(f_\mu)\rangle \mu(\hatzero,\lambda) \binom{\uu}{\lambda} p_\lambda
	&&\text{(by~\eqref{expand-in-P-basis} and~\eqref{Rosas-scalar})}\\
&= \frac{1}{\binom{\uu}{\mu}|\mu|} \sum_\lambda \mu(\hatzero,\lambda) \sum_{\substack{\sigma\colon \type_\uu(\sigma)=\lambda\\ \pi\colon \type_\uu(\pi)=\mu}} \left\langle p_\sigma,\, f_\pi\right\rangle  p_\lambda
	&&\text{(by~\eqref{liftP} and~\eqref{liftF} and bilinearity)}\\
&= \frac{1}{\binom{\uu}{\mu}|\mu|} \sum_\lambda\left[ \mu(\hatzero,\lambda) \sum_{\substack{\sigma\colon \type_\uu(\sigma)=\lambda\\ \pi\colon \type_\uu(\pi)=\mu\\ \pi\leq\sigma}}\sign(\pi)\sign(\sigma)\frac{\mu(\pi,\sigma)}{|\mu(\hatzero,\sigma)|} \right] p_\lambda
	&&\text{(by Doubilet formula \#14)}\\
\end{align*}

\end{document}